wip: subst lemma

TaplLean/STLC/Env.lean
@@ -11,4 +11,34 @@ notation:100 x " |→ " v " ; " τ => update x v τ
 notation:100 x " |→ " v => update x v empty
 
 def sorted {α : Type} (Γ : Env α) (Γ' : Env α) : Prop :=
-  ∀ {x}, Γ x = Γ' x
+  ∀ x, Γ x = Γ' x
+
+theorem sorted_update : ∀ {α : Type} {Γ Γ' : Env α} (x) (v : α),
+  sorted Γ Γ' →
+  sorted (x |→ v ; Γ) (x |→ v ; Γ')
+  := by
+  unfold sorted
+  intro α Γ Γ' x v Hs y
+  unfold update
+  split
+  . rfl
+  . apply Hs
+
+theorem sorted_swap : ∀ {α : Type} (Γ : Env α) (x y vx vy),
+  x ≠ y →
+  sorted (x |→ vx ; y |→ vy ; Γ) (y |→ vy ; x |→ vx ; Γ)
+  := by
+  unfold sorted; intro α Γ x y vx vy Hneq z; unfold update
+  cases String.decEq x z <;> rename_i Hxz
+  . cases String.decEq y z <;> rename_i Hyz
+    . simp [Hxz]
+    . simp [Hxz]
+  . cases String.decEq y z <;> rename_i Hyz
+    . simp [Hxz]; simp [Hyz]
+    . exfalso; rw [← Hyz] at Hxz; apply Hneq Hxz
+
+theorem sorted_extend_eq : ∀ {α : Type} (Γ : Env α) (x v w),
+  sorted (x |→ v ; Γ) (x |→ v ; x |→ w ; Γ)
+  := by
+  intro α Γ x v w y; unfold update
+  cases String.decEq x y <;> rename_i H <;> simp [H]
